ulib/FStar.WellFounded.fst
@@ -12,6 +12,8 @@
    WITHOUT WARRANTIES OR CONDITIONS OF ANY KIND, either express or implied.
    See the License for the specific language governing permissions and
    limitations under the License.
+
+   Authors: Chantal Keller, Catalin Hritcu, Aseem Rastogi, Nikhil Swamy
 *)
 
 (* Defining accessibility predicates and well-founded recursion like in Coq
@@ -20,7 +22,9 @@
 
 module FStar.WellFounded
 
-open FStar.Preorder
+#push-options "--warn_error -242" //inner let recs not encoded to SMT; ok
+
+let binrel (a:Type) = a -> a -> Type
 
 (*
  * The accessibility relation
@@ -30,45 +34,41 @@ open FStar.Preorder
  *)
 [@@ erasable]
 noeq
-type acc (#a:Type) (r:relation a) (x:a) : Type =
+type acc (#a:Type u#a) (r:binrel u#a u#r a) (x:a) : Type u#(max a r) =
   | AccIntro : access_smaller:(y:a -> r y x -> acc r y) -> acc r x
 
 (*
- * A relation r is well-founded if every element is accessible
+ * A binrel r is well-founded if every element is accessible
  *)
-let well_founded (#a:Type) (r:relation a) = x:a -> acc r x
+let well_founded (#a:Type u#a) (r:binrel u#a u#r a) = x:a -> acc r x
 
 (*
  * Accessibility predicates can be used for implementing
  *   total fix points
  *)
-let rec fix_F (#aa:Type) (#r:relation aa) (#p:(aa -> Type))
+let rec fix_F (#aa:Type) (#r:binrel aa) (#p:(aa -> Type))
               (f: (x:aa -> (y:aa -> r y x -> p y) -> p x))
               (x:aa) (a:acc r x)
   : Tot (p x) (decreases a)
   = f x (fun y h -> fix_F f y (a.access_smaller y h))
 
-let fix (#aa:Type) (#r:relation aa) (rwf:well_founded r)
+let fix (#aa:Type) (#r:binrel aa) (rwf:well_founded r)
         (p:aa -> Type) (f:(x:aa -> (y:aa -> r y x -> p y) -> p x))
         (x:aa)
   : p x
   = fix_F f x (rwf x)
 
-let is_well_founded (#a:Type) (rel:relation a) =
+let is_well_founded (#a:Type) (rel:binrel a) =
   forall (x:a). squash (acc rel x)
 
-let well_founded_relation (a:Type) = rel:relation a{is_well_founded rel}
+let well_founded_relation (a:Type) = rel:binrel a{is_well_founded rel}
 
-#push-options "--warn_error -271"
 unfold
-let as_well_founded (#a:Type) (#rel:relation a) (f:(x:a -> acc rel x))
+let as_well_founded (#a:Type) (#rel:binrel a) (f:(x:a -> acc rel x))
   : well_founded_relation a
-  = let aux (x:a)
-      : Lemma (squash (acc rel x))
-              [SMTPat ()]
-      = FStar.Squash.return_squash (f x) in
+  = introduce forall (x:a). acc rel x
+    with FStar.Squash.return_squash (f x);
     rel
-#pop-options
 
 open FStar.IndefiniteDescription
 
@@ -77,8 +77,7 @@ open FStar.IndefiniteDescription
  *
  * Reference: Constructing Recursion Operators in Type Theory, L. Paulson  JSC (1986) 2, 325-355
  *)
-
-let subrelation_wf (#a:Type) (#r #sub_r:relation a)
+let subrelation_wf (#a:Type) (#r #sub_r:binrel a)
   (sub_w:(x:a -> y:a -> sub_r x y -> r x y))
   (r_wf:well_founded r)
   : well_founded sub_r
@@ -89,37 +88,36 @@ let subrelation_wf (#a:Type) (#r #sub_r:relation a)
            | AccIntro f -> f y (sub_w y x sub_r_y_x))) in
     fun x -> aux x (r_wf x)
 
-#push-options "--warn_error -271"
-let subrelation_squash_wf (#a:Type) (#r #sub_r:relation a)
-  (sub_w:(x:a -> y:a -> sub_r x y -> squash (r x y)))
-  (r_wf:well_founded r)
+let subrelation_squash_wf (#a:Type u#a)
+                          (#r:binrel u#a u#r a)
+                          (#sub_r:binrel u#a u#sr a)
+                          (sub_w:(x:a -> y:a -> sub_r x y -> squash (r x y)))
+                          (r_wf:well_founded r)
   : Lemma (is_well_founded sub_r)
-  = let aux (x:a)
-      : Lemma (squash (acc sub_r x))
-              [SMTPat ()]
-      = let rec acc_y (x:a) (acc_r:acc r x) (y:a) (p:sub_r y x)
-          : Tot (acc sub_r y)
-                (decreases acc_r)
-          = AccIntro (acc_y y (acc_r.access_smaller
+  = introduce forall (x:a). squash (acc sub_r x)
+    with (
+      let rec acc_y (x:a) (acc_r:acc r x) (y:a) (p:sub_r y x)
+        : Tot (acc sub_r y)
+              (decreases acc_r)
+        = AccIntro (acc_y y (acc_r.access_smaller
                                    y
-                                   (elim_squash (sub_w y x p)))) in
-        Squash.return_squash (AccIntro (acc_y x (r_wf x)))
-    in
-    ()
-#pop-options
+                                   (elim_squash (sub_w y x p))))
+      in
+      FStar.Squash.return_squash (FStar.Squash.return_squash (AccIntro (acc_y x (r_wf x))))
+    )
 
 unfold
-let subrelation_as_wf (#a:Type) (#r #sub_r:relation a)
+let subrelation_as_wf (#a:Type u#a) (#r #sub_r:binrel u#a u#r a)
   (sub_w:(x:a -> y:a -> sub_r x y -> squash (r x y)))
   (r_wf:well_founded r)
   : well_founded_relation a
   = subrelation_squash_wf sub_w r_wf;
     sub_r
 
-let inverse_image (#a #b:Type) (r_b:relation b) (f:a -> b) : relation a =
+let inverse_image (#a:Type u#a) (#b:Type u#b) (r_b:binrel u#b u#r b) (f:a -> b) : binrel u#a u#r a =
   fun x y -> r_b (f x) (f y)
 
-let inverse_image_wf (#a #b:Type) (#r_b:relation b)
+let inverse_image_wf (#a:Type u#a) (#b:Type u#b) (#r_b:binrel u#b u#r b)
   (f:a -> b)
   (r_b_wf:well_founded r_b)
   : well_founded (inverse_image r_b f)
